Theory: change client to be a process.

RefineDet.thy
@@ -4,6 +4,8 @@ imports Main
 
 begin
 
+section "Process definition. A process represents the computation of a program"
+
 record ('event, 'state, 'external) process =
   Init :: "'external \<Rightarrow> 'state"
   Step :: "'event \<Rightarrow> 'state \<Rightarrow> 'state"
@@ -13,29 +15,52 @@ definition "steps f s events \<equiv> foldl (\<lambda> result event. f event res
 
 definition "exec proc s events \<equiv> (Fin proc) (steps (Step proc) (Init proc s) events)"
 
+section "A model process that simply increments or decrements an integer, and supports viewing it"
+
 datatype E = View | Inc | Dec
 
 definition step :: "E \<Rightarrow> int \<Rightarrow> int" where
 "step e i = (case e of Inc \<Rightarrow> i + 1 | Dec \<Rightarrow> i - 1)"
 
-definition id :: "int \<Rightarrow> int" where
+definition id :: "'a \<Rightarrow> 'a" where
 "id i = i"
 
 definition "Model \<equiv> \<lparr> Init = id, Step = step, Fin = id \<rparr>"
+
+section "An implementation process that has a full-stack web app architecture, with client, server,
+         and application state."
+
+datatype ClientE =
+    ReqInt
+  | RecvInt int
+
+record ClientState =
+  val :: int
+  loading :: bool
+
+definition step_c :: "ClientE \<Rightarrow> ClientState \<Rightarrow> ClientState" where
+"step_c e s =
+ (case e of
+    ReqInt \<Rightarrow> s\<lparr> loading := True \<rparr> 
+  | RecvInt i \<Rightarrow> s\<lparr> loading := False, val := i \<rparr>)"
+
+definition "Client \<equiv> \<lparr> Init = id, Step = step_c, Fin = id \<rparr>"
 
 type_synonym AppState = "(string \<Rightarrow> int)"
 
 record ServerResponse =
   state :: AppState
   response :: int
-  
+
+type_synonym ClientType = "\<lparr> Init :: ClientState \<Rightarrow> ClientState,
+  Step :: ClientE \<Rightarrow> ClientState \<Rightarrow> ClientState,
+  Fin :: ClientState \<Rightarrow> ClientState \<rparr>"
+
 record App = 
-  client :: int 
-  loading :: bool
+  client :: ClientType
+  client_state :: ClientState
   app_state :: AppState
   server :: "E \<Rightarrow> AppState \<Rightarrow> ServerResponse"
-
-(*definition "Client \<equiv> \<lparr> Init = id, Step = step_c, Fin = id \<rparr>" *)
 
 definition app_server :: "E \<Rightarrow> AppState \<Rightarrow> ServerResponse" where
 "app_server r s =
@@ -51,20 +76,25 @@ definition app_server :: "E \<Rightarrow> AppState \<Rightarrow> ServerResponse"
       \<lparr> state = s(''curr_int'' := decd), response = decd \<rparr>)
   )"
 
+definition client_exec :: "E \<Rightarrow> App \<Rightarrow> App" where
+"client_exec e a = (let c = client a in
+         let fetching = exec c (client_state a) [ReqInt] in 
+         let curr_state = app_state a in
+         let resp = (server a) e (app_state a) in
+         let received = exec c fetching [RecvInt ((state resp) ''curr_int'')] in
+           a\<lparr> client_state := received, app_state := state resp \<rparr>)"
+
 definition step_i :: "E \<Rightarrow> App \<Rightarrow> App" where
 "step_i e a = 
   (case e of 
-  Inc => let curr_state = app_state a in
-         let fetching_app = a\<lparr> loading := True \<rparr> in
-         let resp = (server a) e (app_state a) in
-           a\<lparr> client := response resp, loading := False, app_state := state resp \<rparr> |
-  Dec \<Rightarrow> a\<lparr> client := 0, loading := False \<rparr>)"
+  Inc => client_exec e a |
+  Dec \<Rightarrow> client_exec e a)"
 
 definition init_i :: "int \<Rightarrow> App" where
-"init_i i = \<lparr> client = i, loading = False, state = (\<lambda> s. 0), server = app_server \<rparr>"
+"init_i i = \<lparr> client = Client, client_state = \<lparr> val = i, loading = False \<rparr>, app_state = (\<lambda> s. i), server = app_server \<rparr>"
 
 definition fin_i :: "App \<Rightarrow> int" where
-"fin_i as = (if loading as = False then client as else -1)"
+"fin_i a = (if (loading (client_state a)) = False then (val (client_state a)) else -1)"
 
 definition "Impl \<equiv> \<lparr> Init = init_i, Step = step_i, Fin = fin_i \<rparr>"
 
@@ -73,6 +103,12 @@ value "step Inc 1"
 value "steps step 0 [Inc, Inc, Dec, Dec]"
 
 value "exec Model 0 [Inc, Inc]"
+
+value "exec Impl 0 [Inc, Inc]"
+
+value "exec Model (-2) [Dec]"
+
+value "exec Impl (-2) [Dec]"
 
 definition "back_sim S I s events out \<equiv> 
   exec I s events = out \<longrightarrow> exec S s events = out"
@@ -83,7 +119,15 @@ definition "fw_sim S I s events out \<equiv>
 definition "bi_sim S I s events \<equiv> 
   exec I s events = exec S s events"
 
-lemma "bi_sim Model Impl s events"
+lemma "fin_i (step_i e a) = step e (fin_i a)"
+  apply(simp add: fin_i_def step_i_def step_def client_exec_def)
   oops
+
+lemma "bi_sim Model Impl s events"
+  apply(simp add: bi_sim_def exec_def steps_def Impl_def Model_def fin_i_def id_def)
+  oops
+
+  (*apply(unfold bi_sim_def exec_def steps_def Impl_def Model_def) *)
+  (*apply(unfold bi_sim_def exec_def steps_def Impl_def Model_def init_i_def step_i_def fin_i_def id_def step_def client_exec_def)*)
 
 end
